sha3/proof/Utils.ec
@@ -1,0 +1,15 @@
+(** These should make it into the standard libs **)
+require import NewList NewFSet.
+
+op image (f : 'a -> 'b) (X : 'a fset) = oflist (map f (elems X))
+  axiomatized by imageE.
+
+lemma imageP (f : 'a -> 'b) (X : 'a fset) (b : 'b):
+  mem (image f X) b <=> exists a, mem X a /\ f a = b.
+proof.
+  rewrite imageE mem_oflist mapP.
+  (* FIXME *)
+  by split=> [[a] [a_in_X b_def]| [a] [a_in_X b_def]];
+    [rewrite -memE in a_in_X | rewrite memE in a_in_X];
+    exists a; rewrite b_def.
+qed.
